theorems/iN/iN_rewrite.lean
@@ -4,9 +4,9 @@ import theorems.iN.iN_def
 `Rewrite x y` means the value `x` can be rewritten into the value `y`.
 -/
 inductive Rewrite {n} : iN n → iN n → Prop where
-  /-- A non-poison value rewrites to itself. -/
-  | bv_refl (v : BitVec n) : Rewrite (bitvec v) (bitvec v)
-  /-- Poison can be rewritten into any value. -/
+  /-- A value rewrites to itself. -/
+  | refl (x : iN n) : Rewrite x x
+  /-- Poison can be rewritten into any concrete value. -/
   | poison_forge (v : BitVec n) : Rewrite poison (bitvec v)
 
 /--
@@ -23,22 +23,56 @@ abbrev RewriteIff {n} (x y : iN n) := Rewrite x y ∧ Rewrite y x
 @[inherit_doc] infix:50 " <~ "  => RewriteReverse
 @[inherit_doc] infix:50 " <~> " => RewriteIff
 
-/- theorem rewrite_bitvec_iff_equal {n} {x y : BitVec n}
-    : (bitvec x <~> bitvec y) ↔ (x = y) := by
+/-- Poison can be rewritten to anything. -/
+@[simp, grind]
+theorem rewrite_poison {n} (x : iN n)
+    : poison ~> x := by
+
+  cases x
+  case bitvec a =>
+    exact Rewrite.poison_forge a
+  case poison =>
+    exact Rewrite.refl poison
+
+@[refl, simp]
+theorem rewrite_refl {n} {x : iN n}
+    : x <~> x := by
+
+  constructor <;> exact Rewrite.refl x
+
+@[grind →]
+theorem rewrite_trans {n} {x y z : iN n}
+    {hx : x ~> y} {hy : y ~> z} : x ~> z := by
+
+  cases hx
+  case refl =>
+    exact hy
+  case poison_forge v =>
+    exact rewrite_poison z
+
+@[grind]
+theorem eq_rewrite {n} {x y : iN n}
+    : (x = y) → (x <~> y) := by
+
+  intro h
+  rw [h]
+  constructor <;> exact Rewrite.refl y
+
+@[grind]
+theorem eq_iff_rewrite_bitvec {n} {a b : BitVec n}
+    : (a = b) ↔ (bitvec a <~> bitvec b) := by
 
   constructor
   case mp =>
     intro h
-    cases h with
-    | intro hxy hyx =>
-      cases hxy
-      cases hyx
-      rfl
-  case mpr =>
-    intro h
     rw [h]
     constructor
-    case left => exact Rewrite.bv_refl y
-    case right => exact Rewrite.bv_refl y -/
-
--- you can have `poison ~> 12`
+    case left => exact Rewrite.refl (bitvec b)
+    case right => exact Rewrite.refl (bitvec b)
+  case mpr =>
+    intro h
+    cases h with
+    | intro hab hba =>
+      cases hab
+      cases hba
+      rfl
