theorems/iN/iN_lemmas.lean
@@ -1,0 +1,106 @@
+import theorems.iN.SimpSets
+import theorems.iN.iN_def
+import theorems.iN.iN_tactics
+import theorems.iN.iN_rewrite
+import theorems.Core.Attrs.Attrs
+
+@[grind =]
+theorem BitVec.saddOverflow_comm {n} (a b : BitVec n)
+    : a.saddOverflow b = b.saddOverflow a := by
+
+  intros
+  unfold BitVec.saddOverflow
+  grind
+
+@[grind =]
+theorem BitVec.uaddOverflow_comm {n} (a b : BitVec n)
+    : a.uaddOverflow b = b.uaddOverflow a := by
+
+  intros
+  unfold BitVec.uaddOverflow
+  grind
+
+namespace iN
+
+@[grind =]
+theorem addNswBV_comm {n} {a b : BitVec n}
+    : iN.addNswBV a b = iN.addNswBV b a := by
+
+  simp [iN_to_bitvec]
+  rw [BitVec.saddOverflow_comm]
+  split <;> try simp
+
+  -- h✝ : ¬b.saddOverflow a = true
+  -- ⊢ a + b = b + a
+  grind
+
+@[grind =]
+theorem addNuwBV_comm {n} {a b : BitVec n}
+    : iN.addNuwBV a b = iN.addNuwBV b a := by
+
+  simp [iN_to_bitvec]
+  rw [BitVec.uaddOverflow_comm]
+  split <;> try simp
+
+  -- h✝ : ¬b.uaddOverflow a = true
+  -- ⊢ a + b = b + a
+  grind
+
+end iN
+
+/- @[grind =]
+theorem saddOverflow_comm_tete {n} (a b : BitVec n)
+    : a.saddOverflow b = true ↔ b.saddOverflow a = true := by
+
+  unfold BitVec.saddOverflow at *
+  grind -/
+
+/- theorem saddOverflow_contra {n} (a b : BitVec n)
+    :  -/
+
+/- @[simp]
+theorem iN_contra {n} {a : BitVec n}
+    {h : (poison : iN n) = (bitvec a : iN n)} : False := by
+
+  cases h -/
+
+/- theorem test_without {n} (x : iN n) : iN.shlNsw x 0 = x := by
+  simp [iN_unwrap_poison]
+  cases x with
+  | poison => rfl
+  | bitvec a => simp [iN_to_bitvec]
+
+/- theorem com {n} (x y : iN n)
+    : x + y = y + x := by
+
+  cases x with
+  | poison => rfl
+
+  simp [iN_to_bitvec]
+ -/
+
+/- @[simp]
+theorem com {n} (x : iN n) (val : Nat)
+  : ((no_index OfNat.ofNat val) : iN n) + x
+    = x + ((no_index OfNat.ofNat val) : iN n) := by
+  cases x with
+  | poison => rfl
+  | bitvec a =>
+    simp [iN_to_bitvec]
+    apply BitVec.add_comm -/
+
+
+@[simp]
+theorem com0 {n} (x : iN n) (val : Nat)
+  : lit(val) + x = x + lit(val) := by
+  cases x with
+  | poison => rfl
+  | bitvec a =>
+    simp [iN_to_bitvec]
+    apply BitVec.add_comm
+
+-- @bitvec n 23#↑n : iN n
+
+theorem test {n} (x : iN n) : x + x = x + 23 := by
+
+  simp -/
