theorems/iN/iN_tactics.lean
@@ -1,12 +1,40 @@
 import Lean
+import theorems.iN.iN_def
 
 open Lean Elab Tactic Meta
 
-/- elab "lift_poison" : tactic =>
-  Tactic.withMainContext do
-    let goalType ← Lean.Elab.Tactic.getMainTarget
-    dbg_trace f!"goal type: {goalType}"
+-- https://leanprover.zulipchat.com/#narrow/channel/113488-general/topic/Clearing.20obvious.20contradictions.20in.20cases.20of.20goals/near/538579820
 
+/--
+Clears obvious contradictory goals with hypotheses of the form
+`poison = bitvec a` or `bitvec a = poison`.
+-/
+elab "clear_poison_eq" : tactic => do
+  withMainContext do
+    let mainGoal ← getMainGoal
 
-    goalType.eq
- -/
+    let ctx ← getLCtx
+    ctx.forM $ fun (decl : Lean.LocalDecl) => do
+      let declExpr := decl.toExpr
+      let declType ← Lean.Meta.inferType declExpr
+      let (fn, args) := declType.getAppFnArgs
+
+      match fn, args with
+      | `Eq, #[_, lhs, rhs] =>
+
+        -- heq✝ : poison = bitvec a✝
+        -- heq✝ : poison = bitvec b✝
+
+        let isName (e : Expr) (n : Name) : Bool :=
+          e.getAppFn.constName? == some n
+
+        let isPoison (e : Expr) : Bool := isName e ``iN.poison
+        let isBV (e : Expr) : Bool := isName e ``iN.bitvec
+
+        if (isPoison lhs && isBV rhs) || (isPoison rhs && isBV lhs) then
+          let fvarId := decl.fvarId
+          -- clear obvious contradiction
+          let newSubgoals ← mainGoal.cases fvarId
+          replaceMainGoal (newSubgoals.map (·.mvarId)).toList
+          return
+      | _, _ => pure ()
