theorems/iN_basic/add.lean
@@ -1,0 +1,83 @@
+import theorems.iN.iN
+
+namespace iN
+
+-- TODO mark not `@[rewrite]` but something for directional equality
+
+@[grind]
+theorem add_comm {n} (x y : iN n)
+    : x + y = y + x := by
+
+  -- clear poison from `x` and `y`
+  simp only [iN_unwrap_poison]
+  repeat' split; <;> try simp [*] at *
+
+  grind
+
+@[grind]
+theorem addNsw_comm {n} (x y : iN n)
+    : x +nsw y <~> y +nsw x := by
+
+  -- clear poison from `x` and `y`
+  simp only [iN_unwrap_poison]
+
+  cases x
+  . cases y
+    . simp [*] at *
+      grind
+    . simp
+  . simp
+    -- TODO https://leanprover.zulipchat.com/#narrow/channel/113488-general/topic/Simp.20not.20collapsing.20simultaneous.20matching/with/538586043
+    grind
+
+@[grind]
+theorem addNuw_comm {n} (x y : iN n)
+    : x +nuw y <~> y +nuw x := by
+
+  -- clear poison from `x` and `y`
+  simp only [iN_unwrap_poison]
+
+  cases x
+  . cases y
+    . simp [*] at *
+      grind
+    . simp
+  . simp
+    -- TODO https://leanprover.zulipchat.com/#narrow/channel/113488-general/topic/Simp.20not.20collapsing.20simultaneous.20matching/with/538586043
+    grind
+
+@[grind]
+theorem add_assoc {n} (x y z : iN n)
+    : (x + y) + z = x + (y + z) := by
+
+  -- clear poison from `x` and `y`
+  simp only [iN_unwrap_poison]
+
+  cases x
+  . cases y
+    . cases z
+      . simp
+        grind
+      . simp
+    . simp
+  . simp
+
+/- @[grind]
+theorem addNsw_assoc {n} (x y z : iN n)
+    : (x +nsw y) +nsw z <~> x +nsw (y +nsw z) := by
+
+  -- clear poison from `x` and `y`
+  simp only [iN_unwrap_poison]
+
+  cases x
+  . cases y
+    . cases z
+      . simp
+
+
+
+      . simp
+    . simp
+  . simp -/
+
+end iN
