theorems/iN_normal/iN_normal.lean
@@ -1,1 +1,0 @@
-import theorems.iN_normal.tilde
